theories/tactics.v
@@ -1,0 +1,118 @@
+From iris.proofmode Require Import base tactics classes.
+From hazel          Require Export weakestpre.
+
+
+(* The tactic [reshape_expr] was taken from
+   Tej Chajed's [iris-simp-lang] GitHub repository.
+ *)
+Ltac reshape_expr e tac :=
+  let rec go K e :=
+    match e with
+    | Do ?e                 => add_item DoCtx K e
+    | App ?e (Val ?v)       => add_item (AppLCtx v) K e
+    | App ?e1 ?e2           => add_item (AppRCtx e1) K e2
+    | UnOp ?op ?e           => add_item (UnOpCtx op) K e
+    | BinOp ?op ?e (Val ?v) => add_item (BinOpLCtx op v) K e
+    | BinOp ?op ?e1 ?e2     => add_item (BinOpRCtx op e1) K e2
+    | If ?e0 ?e1 ?e2        => add_item (IfCtx e1 e2) K e0
+    | Pair ?e (Val ?v)      => add_item (PairLCtx v) K e
+    | Pair ?e1 ?e2          => add_item (PairRCtx e1) K e2
+    | Fst ?e                => add_item FstCtx K e
+    | Snd ?e                => add_item SndCtx K e
+    | InjL ?e               => add_item InjLCtx K e
+    | InjR ?e               => add_item InjRCtx K e
+    | Case ?e0 ?e1 ?e2      => add_item (CaseCtx e1 e2) K e0
+    | Alloc ?e              => add_item AllocCtx K e
+    | Load ?e               => add_item LoadCtx K e
+    | Store ?e (Val ?v)     => add_item (StoreLCtx v) K e
+    | Store ?e1 ?e2         => add_item (StoreRCtx e1) K e2
+
+    | Val _                 => tac K e
+    | Eff _ _               => tac K e
+    | TryWith _ _ _         => tac K e
+    | Var _                 => tac K e
+    | Rec _ _ _             => tac K e
+  end
+  with add_item Ki K e := go (ConsCtx Ki K) e
+  in go EmptyCtx e.
+
+Ltac match_ewp_goal tac :=
+  match goal with
+  | [ |- @bi_emp_valid _                (ewp_def ?E ?e ?Ψ ?ϕ) ] => tac E e Ψ ϕ
+  | [ |- @environments.envs_entails _ _ (ewp_def ?E ?e ?Ψ ?ϕ) ] => tac E e Ψ ϕ
+  end.
+
+Ltac ewp_bind_rule_tac _ e _ _ :=
+  let reverse_ctx K :=
+    let rec go acc K :=
+      match K with
+      | EmptyCtx       => acc
+      | ConsCtx ?Ki ?K => go (ConsCtx Ki acc) K
+      end
+    in
+    go EmptyCtx K
+  in
+
+  let apply_bind_rule K :=
+    match K with
+    | EmptyCtx    => idtac
+    | ConsCtx _ _ =>
+       let K := reverse_ctx K in
+       iApply (ewp_bind    K); [done|]
+    end
+  in
+
+  let tac K e :=
+    match e with
+    | Val ?v =>
+       match K with
+       | EmptyCtx      => idtac
+       | ConsCtx  _ ?K => apply_bind_rule K
+       end
+    | _ => apply_bind_rule K
+    end
+  in
+
+  reshape_expr e tac.
+
+Ltac ewp_pure_step_tac _ e _ _ :=
+  match e with
+  | Val _ =>
+     iApply ewp_value
+  | TryWith (Val _) _ _ =>
+     iApply (ewp_pure_step'); [apply pure_prim_step_try_with_val|]
+  | Rec _ _ _ =>
+     iApply (ewp_pure_step'); [apply pure_prim_step_rec|]
+  | App (Val (RecV _ _ _)) (Val _) =>
+     iApply (ewp_pure_step'); [apply pure_prim_step_beta|]
+  | UnOp _ _ =>
+     iApply (ewp_pure_step'); [apply pure_prim_step_unop|]
+  | BinOp _ _ _ =>
+     iApply (ewp_pure_step'); [apply pure_prim_step_binop|]
+  | If (Val (LitV (LitBool _))) _ _ =>
+     iApply (ewp_pure_step'); [apply pure_prim_step_if|]
+  | Pair (Val _) (Val _) =>
+     iApply (ewp_pure_step'); [apply pure_prim_step_pair|]
+  | Fst (Val (PairV _ _)) =>
+     iApply (ewp_pure_step'); [apply pure_prim_step_Fst|]
+  | Snd (Val (PairV _ _)) =>
+     iApply (ewp_pure_step'); [apply pure_prim_step_Snd|]
+  | InjL (Val _) =>
+     iApply (ewp_pure_step'); [apply pure_prim_step_InjL|]
+  | InjR (Val _) =>
+     iApply (ewp_pure_step'); [apply pure_prim_step_InjR|]
+  | Case (Val (InjLV _)) _ _ =>
+     iApply (ewp_pure_step'); [apply pure_prim_step_case_InjL|]
+  | Case (Val (InjRV _)) _ _ =>
+     iApply (ewp_pure_step'); [apply pure_prim_step_case_InjR|]
+  end.
+
+Ltac ewp_bind_rule :=
+  match_ewp_goal ewp_bind_rule_tac.
+
+Ltac ewp_pure_step :=
+  match_ewp_goal ewp_pure_step_tac.
+
+Ltac ewp_pure_steps :=
+  repeat (ewp_bind_rule; simpl;
+          ewp_pure_step; try iNext; simpl).
